# Test1 Review Material {-}

Below are resources to help you practice and prepare for the test 2 in this course.

Test 2 will cover the material covered in Chapter 4 of this textbook:

- basic derivative rules
- product, quotient and chain rules
- implicit derivatives

What's not on this test:

- no interpretation style questions on this test
- no derivations 
- no limit definitions

## Test Instructions {-}
Below are the general instructions for all tests

- You will get a chance to **retake** this. Your **highest** score counts toward your final grade.  
- Follow the guidance for each part and **show all work** for full credit.  
- **Non-graphical calculators** are allowed.  
- **One page (two sides)** of handwritten (or font size 8) notes are allowed.
- The equation sheet from the textbook is included as part of the test pack (it doesn't count as note pages)

## Basic Rule Practice

### 1. \(f(x)=7\){-}

<details>
<summary><strong>Math Hint</strong></summary>
The derivative of any constant is always \(0\).  
Think of a flat line — its slope never changes.
</details>

<details>
<summary><strong>Solution</strong></summary>
\(f'(x)=0\)
</details>

---

### 2. \(f(x)=x^5\){-}

<details>
<summary><strong>Math Hint</strong></summary>
Use the **power rule**: \((x^n)' = n x^{n-1}\).
</details>

<details>
<summary><strong>Solution</strong></summary>
\(f'(x)=5x^4\)
</details>

---

### 3. \(f(x)=3x^4\){-}

<details>
<summary><strong>Math Hint</strong></summary>
You have a constant multiplied by a power of \(x\).  
Apply the **constant multiple rule** with the **power rule**.
</details>

<details>
<summary><strong>Solution</strong></summary>
\(f'(x)=12x^3\)
</details>

---

### 4. \(f(x)=5x^3-2x^2\){-}

<details>
<summary><strong>Math Hint</strong></summary>
Use the **difference rule**: differentiate each term individually.
</details>

<details>
<summary><strong>Solution</strong></summary>
\(f'(x)=15x^2-4x\)
</details>

---

### 5. \(f(x)=x^4+3x^2+5\){-}

<details>
<summary><strong>Math Hint</strong></summary>
Use the **sum rule** and note that the derivative of a constant is zero.
</details>

<details>
<summary><strong>Solution</strong></summary>
\(f'(x)=4x^3+6x\)
</details>

---

### 6. \(f(x)=9x^7-4x^3+2x\){-}

<details>
<summary><strong>Math Hint</strong></summary>
Each term loses one power when you apply the power rule.
</details>

<details>
<summary><strong>Solution</strong></summary>
\(f'(x)=63x^6-12x^2+2\)
</details>

---

### 7. \(f(x)=\dfrac{1}{2}x^2-3x+4\){-}

<details>
<summary><strong>Math Hint</strong></summary>
Differentiate each term.  
The first term is a parabola — its slope changes linearly with \(x\).
</details>

<details>
<summary><strong>Solution</strong></summary>
\(f'(x)=x-3\)
</details>

---

### 8. \(f(x)=10x^3+7x-12\){-}

<details>
<summary><strong>Math Hint</strong></summary>
Differentiate each term using the power rule.
</details>

<details>
<summary><strong>Solution</strong></summary>
\(f'(x)=30x^2+7\)
</details>

---

### 9. \(f(x)=x^6-9x^2+1\){-}

<details>
<summary><strong>Math Hint</strong></summary>
Find \(f'(x)\) and simplify.
</details>

<details>
<summary><strong>Solution</strong></summary>
\(f'(x)=6x^5-18x=6x(x^4-3)\)
</details>

---

### 10. \(f(x)=4x^3-12x^2+9x-1\){-}

<details>
<summary><strong>Math Hint</strong></summary>
Differentiate each term; the derivative of a cubic is a quadratic.
</details>

<details>
<summary><strong>Solution</strong></summary>
\(f'(x)=12x^2-24x+9\)
</details>

---

## Identity Rule Practice

### 1. \(f(x)=e^x\){-}

<details>
<summary><strong>Math Hint</strong></summary>
The derivative of \(e^x\) is itself.
</details>

<details>
<summary><strong>Solution</strong></summary>
\(f'(x)=e^x\)
</details>

---

### 2. \(f(x)=3e^x\){-}

<details>
<summary><strong>Math Hint</strong></summary>
Use the constant multiple rule.
</details>

<details>
<summary><strong>Solution</strong></summary>
\(f'(x)=3e^x\)
</details>

---

### 3. \(f(x)=2e^{2x}\){-}

<details>
<summary><strong>Math Hint</strong></summary>
Use \( (e^{g(x)})' = g'(x)e^{g(x)} \).
</details>

<details>
<summary><strong>Solution</strong></summary>
\(f'(x)=4e^{2x}\)
</details>

---

### 4. \(f(x)=5e^{-x}\){-}

<details>
<summary><strong>Math Hint</strong></summary>
For \(g(x)=-x\), \(g'(x)=-1\).
</details>

<details>
<summary><strong>Solution</strong></summary>
\(f'(x)=-5e^{-x}\)
</details>

---

### 5. \(f(x)=e^{x^2}\){-}

<details>
<summary><strong>Math Hint</strong></summary>
Use \( (e^{g(x)})' = g'(x)e^{g(x)} \).
</details>

<details>
<summary><strong>Solution</strong></summary>
\(f'(x)=2x e^{x^2}\)
</details>

---

### 6. \(f(x)=e^{3x+1}\){-}

<details>
<summary><strong>Math Hint</strong></summary>
Differentiate the exponent \(3x+1\).
</details>

<details>
<summary><strong>Solution</strong></summary>
\(f'(x)=3e^{3x+1}\)
</details>

---

### 7. \(f(x)=10^x\){-}

<details>
<summary><strong>Math Hint</strong></summary>
Use \( (a^x)' = a^x \ln(a) \).
</details>

<details>
<summary><strong>Solution</strong></summary>
\(f'(x)=10^x \ln(10)\)
</details>

---

### 8. \(f(x)=2^{3x}\){-}

<details>
<summary><strong>Math Hint</strong></summary>
Use \( (a^{g(x)})' = g'(x)a^{g(x)}\ln(a) \).
</details>

<details>
<summary><strong>Solution</strong></summary>
\(f'(x)=3(2^{3x}\ln 2)\)
</details>

---

### 9. \(f(x)=5^x + 7^x\){-}

<details>
<summary><strong>Math Hint</strong></summary>
Differentiate each term individually.
</details>

<details>
<summary><strong>Solution</strong></summary>
\(f'(x)=5^x\ln(5)+7^x\ln(7)\)
</details>

---

### 10. \(f(x)=3^x - 2^x\){-}

<details>
<summary><strong>Math Hint</strong></summary>
Use \(a^x\ln(a)\) for each term.
</details>

<details>
<summary><strong>Solution</strong></summary>
\(f'(x)=3^x\ln(3)-2^x\ln(2)\)
</details>

---

### 11. \(f(x)=\ln(x)\){-}

<details>
<summary><strong>Math Hint</strong></summary>
Derivative of \(\ln(x)\) is \(1/x\).
</details>

<details>
<summary><strong>Solution</strong></summary>
\(f'(x)=\dfrac{1}{x}\)
</details>

---

### 12. \(f(x)=\ln(3x)\){-}

<details>
<summary><strong>Math Hint</strong></summary>
Use chain rule with \(g(x)=3x\).
</details>

<details>
<summary><strong>Solution</strong></summary>
\(f'(x)=\dfrac{1}{x}\)
</details>

---

### 13. \(f(x)=\ln(x^2+1)\){-}

<details>
<summary><strong>Math Hint</strong></summary>
Use \((\ln g(x))'=\dfrac{g'(x)}{g(x)}\).
</details>

<details>
<summary><strong>Solution</strong></summary>
\(f'(x)=\dfrac{2x}{x^2+1}\)
</details>

---

### 14. \(f(x)=\ln(\sqrt{x})\){-}

<details>
<summary><strong>Math Hint</strong></summary>
\(\sqrt{x}=x^{1/2}\)
</details>

<details>
<summary><strong>Solution</strong></summary>
\(f'(x)=\dfrac{1}{2x}\)
</details>

---

### 15. \(f(x)=\log_2(x)\){-}

<details>
<summary><strong>Math Hint</strong></summary>
\((\log_a x)'=\dfrac{1}{x\ln(a)}\)
</details>

<details>
<summary><strong>Solution</strong></summary>
\(f'(x)=\dfrac{1}{x\ln(2)}\)
</details>

---

### 16. \(f(x)=\log_3(2x)\){-}

<details>
<summary><strong>Math Hint</strong></summary>
Use chain rule with \((\log_a(g(x)))'=\dfrac{g'(x)}{g(x)\ln(a)}\).
</details>

<details>
<summary><strong>Solution</strong></summary>
\(f'(x)=\dfrac{1}{x\ln(3)}\)
</details>

---

### 17. \(f(x)=\ln(e^x+1)\){-}

<details>
<summary><strong>Math Hint</strong></summary>
Use chain rule with \(g(x)=e^x+1\).
</details>

<details>
<summary><strong>Solution</strong></summary>
\(f'(x)=\dfrac{e^x}{e^x+1}\)
</details>

---

### 18. \(f(x)=e^{\ln(x)}\){-}

<details>
<summary><strong>Math Hint</strong></summary>
Simplify \(e^{\ln(x)}=x\).
</details>

<details>
<summary><strong>Solution</strong></summary>
\(f'(x)=1\)
</details>

---

### 19. \(f(x)=x e^x\){-}

<details>
<summary><strong>Math Hint</strong></summary>
Use product rule.
</details>

<details>
<summary><strong>Solution</strong></summary>
\(f'(x)=e^x(1+x)\)
</details>

---

### 20. \(f(x)=x\ln(x)\){-}

<details>
<summary><strong>Math Hint</strong></summary>
Use product rule.
</details>

<details>
<summary><strong>Solution</strong></summary>
\(f'(x)=\ln(x)+1\)
</details>

---
